CppFormalization/Cpp4/Resource/All.lean
@@ -1,5 +1,5 @@
 import CppFormalization.Cpp4.Resource.Capability
-import CppFormalization.Cpp4.Resource.Demand
-import CppFormalization.Cpp4.Resource.Effect
-import CppFormalization.Cpp4.Resource.Noninterference
-import CppFormalization.Cpp4.Resource.Transport
+import CppFormalization.Cpp4.Resource.Demand.All
+import CppFormalization.Cpp4.Resource.Effect.All
+import CppFormalization.Cpp4.Resource.Noninterference.All
+import CppFormalization.Cpp4.Resource.Transport.All
